secp256k1: move precomputed table to a static header

code/k256/Hacl.Impl.K256.PointMul.fst
@@ -10,201 +10,22 @@ open Lib.Buffer
 module ST = FStar.HyperStack.ST
 module LSeq = Lib.Sequence
 
-module LE = Lib.Exponentiation
 module SE = Spec.Exponentiation
 module BE = Hacl.Impl.Exponentiation
 module ME = Hacl.Impl.MultiExponentiation
 module PT = Hacl.Impl.PrecompTable
-module SPT = Hacl.Spec.PrecompBaseTable
 
 module S = Spec.K256
-module SL = Spec.K256.Lemmas
 
-open Hacl.K256.Field
 open Hacl.K256.Scalar
 open Hacl.Impl.K256.Point
+include Hacl.Impl.K256.Group
+include Hacl.K256.PrecompTable
 
 #set-options "--z3rlimit 50 --fuel 0 --ifuel 0"
 
-///////////////////////////////////////////
-
-unfold
-let linv_ctx (a:LSeq.lseq uint64 0) : Type0 = True
-
-unfold
-let refl (p:LSeq.lseq uint64 15{point_inv_lseq p}) : GTot S.aff_point =
-  S.to_aff_point (point_eval_lseq p)
-
 inline_for_extraction noextract
-let mk_to_k256_comm_monoid : BE.to_comm_monoid U64 15ul 0ul = {
-  BE.a_spec = S.aff_point;
-  BE.comm_monoid = S.mk_k256_comm_monoid;
-  BE.linv_ctx = linv_ctx;
-  BE.linv = point_inv_lseq;
-  BE.refl = refl;
-  }
-
-
-inline_for_extraction noextract
-val point_add : BE.lmul_st U64 15ul 0ul mk_to_k256_comm_monoid
-let point_add ctx x y xy =
-  let h0 = ST.get () in
-  SL.to_aff_point_add_lemma (point_eval h0 x) (point_eval h0 y);
-  Hacl.Impl.K256.PointAdd.point_add xy x y
-
-
-inline_for_extraction noextract
-val point_double : BE.lsqr_st U64 15ul 0ul mk_to_k256_comm_monoid
-let point_double ctx x xx =
-  let h0 = ST.get () in
-  SL.to_aff_point_double_lemma (point_eval h0 x);
-  Hacl.Impl.K256.PointDouble.point_double xx x
-
-
-val make_point_at_inf: p:point -> Stack unit
-  (requires fun h -> live h p)
-  (ensures  fun h0 _ h1 -> modifies (loc p) h0 h1 /\
-    point_inv h1 p /\ S.to_aff_point (point_eval h1 p) == S.aff_point_at_inf)
-
-let make_point_at_inf p =
-  SL.to_aff_point_at_infinity_lemma ();
-  let px, py, pz = getx p, gety p, getz p in
-  set_zero px;
-  set_one py;
-  set_zero pz
-
-
-inline_for_extraction noextract
-val point_zero : BE.lone_st U64 15ul 0ul mk_to_k256_comm_monoid
-let point_zero ctx one = make_point_at_inf one
-
-
-inline_for_extraction noextract
-let mk_k256_concrete_ops : BE.concrete_ops U64 15ul 0ul = {
-  BE.to = mk_to_k256_comm_monoid;
-  BE.lone = point_zero;
-  BE.lmul = point_add;
-  BE.lsqr = point_double;
-}
-
-//////////////////////////////////////////////////////
-
-inline_for_extraction noextract
-val proj_point_to_list: p:S.proj_point
-  -> x:list uint64{FStar.List.Tot.length x = 15 /\
-    mk_to_k256_comm_monoid.BE.linv (Seq.seq_of_list x)}
-
-let proj_point_to_list p =
-  Hacl.Spec.K256.PrecompTable.proj_point_to_list_lemma p;
-  Hacl.Spec.K256.PrecompTable.proj_point_to_list p
-
-val lemma_refl: x:S.proj_point ->
-  Lemma (S.mk_k256_concrete_ops.SE.to.SE.refl x ==
-    mk_to_k256_comm_monoid.BE.refl (Seq.seq_of_list (proj_point_to_list x)))
-
-let lemma_refl x =
-  assert (S.mk_k256_concrete_ops.SE.to.SE.refl x == S.to_aff_point x);
-  assert (mk_to_k256_comm_monoid.BE.refl (Seq.seq_of_list (proj_point_to_list x)) ==
-    S.to_aff_point (point_eval_lseq (Seq.seq_of_list (proj_point_to_list x))));
-  Hacl.Spec.K256.PrecompTable.proj_point_to_list_eval x;
-  assert (Hacl.Spec.K256.PrecompTable.point_eval_list (proj_point_to_list x) == x);
-  assert (point_eval_lseq (Seq.seq_of_list (proj_point_to_list x)) == x)
-
-
-inline_for_extraction noextract
-let mk_k256_precomp_base_table: SPT.mk_precomp_base_table S.proj_point U64 15ul 0ul = {
-  SPT.concr_ops = S.mk_k256_concrete_ops;
-  SPT.to_cm = mk_to_k256_comm_monoid;
-  SPT.to_list = proj_point_to_list;
-  SPT.lemma_refl = lemma_refl;
-}
-
-unfold let precomp_basepoint_table_list: x:list uint64{FStar.List.Tot.length x = 240} =
-  normalize_term (SPT.precomp_base_table_list mk_k256_precomp_base_table S.g 15)
-
-inline_for_extraction noextract
-let precomp_basepoint_table_lseq : LSeq.lseq uint64 240 =
-  normalize_term_spec (SPT.precomp_base_table_list mk_k256_precomp_base_table S.g 15);
-  Seq.seq_of_list precomp_basepoint_table_list
-
-inline_for_extraction noextract
-let pow_base_point (k:nat) =
-  LE.pow S.mk_k256_comm_monoid (S.to_aff_point S.g) k
-
-unfold
-let precomp_table_acc_inv
-  (table_len:nat{table_len * 15 <= max_size_t})
-  (table:LSeq.lseq uint64 (table_len * 15))
-  (j:nat{j < table_len})
-=
-  Math.Lemmas.lemma_mult_lt_right 15 j table_len;
-  Math.Lemmas.lemma_mult_le_right 15 (j + 1) table_len;
-  let bj = LSeq.sub table (j * 15) 15 in
-  point_inv_lseq bj /\ S.to_aff_point (point_eval_lseq bj) == pow_base_point j
-
-val precomp_basepoint_table_lemma: unit ->
-  Lemma (forall (i:nat{i < 16}). precomp_table_acc_inv 16 precomp_basepoint_table_lseq i)
-let precomp_basepoint_table_lemma () =
-  normalize_term_spec (SPT.precomp_base_table_list mk_k256_precomp_base_table S.g 15);
-  SPT.precomp_base_table_lemma mk_k256_precomp_base_table S.g 16 precomp_basepoint_table_lseq
-
-/////////////////////////////////////////////////////
-
-inline_for_extraction noextract
-val make_g: g:point -> Stack unit
-  (requires fun h -> live h g)
-  (ensures  fun h0 _ h1 -> modifies (loc g) h0 h1 /\
-    point_inv h1 g /\ point_eval h1 g == S.g)
-
-let make_g g =
-  let gx, gy, gz = getx g, gety g, getz g in
-
-  [@inline_let]
-  let x =
-   (u64 0x2815b16f81798,
-    u64 0xdb2dce28d959f,
-    u64 0xe870b07029bfc,
-    u64 0xbbac55a06295c,
-    u64 0x79be667ef9dc) in
-
-  assert_norm (0x79be667ef9dc < max48);
-  assert_norm (0xe1108a8fd17b4 < max52);
-  assert_norm (S.g_x == as_nat5 x);
-  make_u52_5 gx x;
-
-  [@inline_let]
-  let y =
-   (u64 0x7d08ffb10d4b8,
-    u64 0x48a68554199c4,
-    u64 0xe1108a8fd17b4,
-    u64 0xc4655da4fbfc0,
-    u64 0x483ada7726a3) in
-
-  assert_norm (S.g_y == as_nat5 y);
-  make_u52_5 gy y;
-
-  set_one gz
-
-
-val point_mul: out:point -> scalar:qelem -> q:point -> Stack unit
-  (requires fun h ->
-    live h out /\ live h scalar /\ live h q /\
-    disjoint out q /\ disjoint out scalar /\ disjoint q scalar /\
-    point_inv h q /\ qas_nat h scalar < S.q)
-  (ensures  fun h0 _ h1 -> modifies (loc out) h0 h1 /\
-    point_inv h1 out /\
-    S.to_aff_point (point_eval h1 out) ==
-    S.to_aff_point (S.point_mul (qas_nat h0 scalar) (point_eval h0 q)))
-
-let point_mul out scalar q =
-  let h0 = ST.get () in
-  SE.exp_fw_lemma S.mk_k256_concrete_ops (point_eval h0 q) 256 (qas_nat h0 scalar) 4;
-  BE.lexp_fw_consttime 15ul 0ul mk_k256_concrete_ops 4ul (null uint64) q 4ul 256ul scalar out
-
-////////////////////////////////////////
-
-inline_for_extraction noextract
-let table_inv : BE.table_inv_t U64 15ul 16ul =
+let table_inv_w4 : BE.table_inv_t U64 15ul 16ul =
   [@inline_let] let len = 15ul in
   [@inline_let] let ctx_len = 0ul in
   [@inline_let] let k = mk_k256_concrete_ops in
@@ -212,10 +33,22 @@ let table_inv : BE.table_inv_t U64 15ul 16ul =
   [@inline_let] let table_len = 16ul in
   BE.table_inv_precomp len ctx_len k l table_len
 
+(*
+inline_for_extraction noextract
+let table_inv_w5 : BE.table_inv_t U64 15ul 32ul =
+  [@inline_let] let len = 15ul in
+  [@inline_let] let ctx_len = 0ul in
+  [@inline_let] let k = mk_k256_concrete_ops in
+  [@inline_let] let l = 5ul in
+  [@inline_let] let table_len = 32ul in
+  assert_norm (pow2 (v l) == v table_len);
+  BE.table_inv_precomp len ctx_len k l table_len
+*)
 
-let precomp_basepoint_table:
-  x:glbuffer uint64 240ul{witnessed x precomp_basepoint_table_lseq /\ recallable x} =
-  createL_global precomp_basepoint_table_list
+let point_mul out scalar q =
+  let h0 = ST.get () in
+  SE.exp_fw_lemma S.mk_k256_concrete_ops (point_eval h0 q) 256 (qas_nat h0 scalar) 4;
+  BE.lexp_fw_consttime 15ul 0ul mk_k256_concrete_ops 4ul (null uint64) q 4ul 256ul scalar out
 
 
 inline_for_extraction noextract
@@ -242,26 +75,17 @@ let point_mul_g_noalloc out scalar g =
   let h0 = ST.get () in
   SE.exp_fw_lemma S.mk_k256_concrete_ops (point_eval h0 g) 256 (qas_nat h0 scalar) 4;
 
-  recall_contents precomp_basepoint_table precomp_basepoint_table_lseq;
+  recall_contents precomp_basepoint_table_w4 precomp_basepoint_table_lseq_w4;
   let h1 = ST.get () in
-  precomp_basepoint_table_lemma ();
-  assert (table_inv (as_seq h1 g) (as_seq h1 precomp_basepoint_table));
+  precomp_basepoint_table_lemma_w4 ();
+  assert (table_inv_w4 (as_seq h1 g) (as_seq h1 precomp_basepoint_table_w4));
   assert (point_eval h1 g == S.g);
 
   BE.mk_lexp_fw_table len ctx_len k l table_len
-    table_inv
+    table_inv_w4
     (BE.lprecomp_get_consttime len ctx_len k l table_len)
-    (null uint64) g bLen bBits scalar (to_const precomp_basepoint_table) out
+    (null uint64) g bLen bBits scalar (to_const precomp_basepoint_table_w4) out
 
-
-val point_mul_g: out:point -> scalar:qelem -> Stack unit
-  (requires fun h ->
-    live h scalar /\ live h out /\ disjoint out scalar /\
-    qas_nat h scalar < S.q)
-  (ensures  fun h0 _ h1 -> modifies (loc out) h0 h1 /\
-    point_inv h1 out /\
-    S.to_aff_point (point_eval h1 out) ==
-    S.to_aff_point (S.point_mul_g (qas_nat h0 scalar)))
 
 [@CInline]
 let point_mul_g out scalar =
@@ -271,6 +95,7 @@ let point_mul_g out scalar =
   point_mul_g_noalloc out scalar g;
   pop_frame ()
 
+//-------------------------
 
 inline_for_extraction noextract
 val point_mul_g_double_vartime_noalloc:
@@ -288,7 +113,7 @@ val point_mul_g_double_vartime_noalloc:
 
     qas_nat h scalar1 < S.q /\ qas_nat h scalar2 < S.q /\
     point_inv h q1 /\ point_eval h q1 == S.g /\ point_inv h q2 /\
-    table_inv (as_seq h q2) (as_seq h table2))
+    table_inv_w4 (as_seq h q2) (as_seq h table2))
   (ensures fun h0 _ h1 -> modifies (loc out) h0 h1 /\
     point_inv h1 out /\
     S.to_aff_point (point_eval h1 out) ==
@@ -305,35 +130,23 @@ let point_mul_g_double_vartime_noalloc out scalar1 q1 scalar2 q2 table2 =
   [@inline_let] let bBits = 256ul in
 
   let h0 = ST.get () in
-  recall_contents precomp_basepoint_table precomp_basepoint_table_lseq;
+  recall_contents precomp_basepoint_table_w4 precomp_basepoint_table_lseq_w4;
   let h1 = ST.get () in
-  precomp_basepoint_table_lemma ();
-  assert (table_inv (as_seq h1 q1) (as_seq h1 precomp_basepoint_table));
-  assert (table_inv (as_seq h1 q2) (as_seq h1 table2));
+  precomp_basepoint_table_lemma_w4 ();
+  assert (table_inv_w4 (as_seq h1 q1) (as_seq h1 precomp_basepoint_table_w4));
+  assert (table_inv_w4 (as_seq h1 q2) (as_seq h1 table2));
 
   ME.mk_lexp_double_fw_tables len ctx_len k l table_len
-    table_inv table_inv
+    table_inv_w4 table_inv_w4
     (BE.lprecomp_get_vartime len ctx_len k l table_len)
     (BE.lprecomp_get_vartime len ctx_len k l table_len)
     (null uint64) q1 bLen bBits scalar1 q2 scalar2
-    (to_const precomp_basepoint_table) (to_const table2) out;
+    (to_const precomp_basepoint_table_w4) (to_const table2) out;
 
   SE.exp_double_fw_lemma S.mk_k256_concrete_ops
     (point_eval h0 q1) 256 (qas_nat h0 scalar1)
     (point_eval h0 q2) (qas_nat h0 scalar2) 4
 
-
-val point_mul_g_double_vartime: out:point -> scalar1:qelem -> scalar2:qelem -> q2:point ->
-  Stack unit
-  (requires fun h ->
-    live h out /\ live h scalar1 /\ live h scalar2 /\ live h q2 /\
-    disjoint q2 out /\ disjoint out scalar1 /\ disjoint out scalar2 /\
-    point_inv h q2 /\ qas_nat h scalar1 < S.q /\ qas_nat h scalar2 < S.q)
-  (ensures fun h0 _ h1 -> modifies (loc out) h0 h1 /\
-    point_inv h1 out /\
-    S.to_aff_point (point_eval h1 out) ==
-    S.to_aff_point (S.point_mul_double_g
-      (qas_nat h0 scalar1) (qas_nat h0 scalar2) (point_eval h0 q2)))
 
 [@CInline]
 let point_mul_g_double_vartime out scalar1 scalar2 q2 =
@@ -348,6 +161,7 @@ let point_mul_g_double_vartime out scalar1 scalar2 q2 =
 
   let table2 = create (table_len *! len) (u64 0) in
   PT.lprecomp_table len ctx_len k (null uint64) q2 table_len table2;
-
+  let h = ST.get () in
+  assert (table_inv_w4 (as_seq h q2) (as_seq h table2));
   point_mul_g_double_vartime_noalloc out scalar1 q1 scalar2 q2 table2;
   pop_frame ()
