code/k256/Hacl.Spec.K256.PrecompTable.fst
@@ -13,32 +13,6 @@ module SPT = Hacl.Spec.PrecompBaseTable
 
 #set-options "--z3rlimit 50 --fuel 0 --ifuel 0"
 
-unfold
-let create5 (x0 x1 x2 x3 x4:uint64) : list uint64 = [x0; x1; x2; x3; x4]
-
-inline_for_extraction noextract
-let felem_list = x:list uint64{FL.length x == 5}
-inline_for_extraction noextract
-let point_list = x:list uint64{FL.length x == 15}
-
-inline_for_extraction noextract
-let felem_to_list (x:S.felem) : felem_list =
-  [@inline_let] let x0 = x % pow52 in
-  [@inline_let] let x1 = x / pow52 % pow52 in
-  [@inline_let] let x2 = x / pow104 % pow52 in
-  [@inline_let] let x3 = x / pow156 % pow52 in
-  [@inline_let] let x4 = x / pow208 in
-  [@inline_let] let r = create5 (u64 x0) (u64 x1) (u64 x2) (u64 x3) (u64 x4) in
-  assert_norm (FL.length r = 5);
-  r
-
-inline_for_extraction noextract
-let proj_point_to_list (p:S.proj_point) : point_list =
-  [@inline_let] let (px, py, pz) = p in
-  FL.(felem_to_list px @ felem_to_list py @ felem_to_list pz)
-
-//----------------------------------------------
-
 let create5_lseq (x0 x1 x2 x3 x4:uint64) : lseq uint64 5 =
   let l = [x0; x1; x2; x3; x4] in
   assert_norm (FL.length l = 5);
@@ -143,17 +117,6 @@ let felem_to_list_lemma_eval x =
 
 //--------------------------------------------
 
-inline_for_extraction noextract
-let point_inv_list (p:point_list) =
-  let x = Seq.seq_of_list p <: lseq uint64 15 in
-  point_inv_lseq x
-
-noextract
-let point_eval_list (p:point_list) : GTot S.proj_point =
-  let x = Seq.seq_of_list p <: lseq uint64 15 in
-  point_eval_lseq x
-
-
 val proj_point_to_list_sub: p:S.proj_point -> Lemma
  (let (px, py, pz) = p in
   let px_list = felem_to_list px in
@@ -204,9 +167,6 @@ let proj_point_to_list_eval p =
   Math.Lemmas.small_mod py S.prime;
   Math.Lemmas.small_mod pz S.prime
 
-
-val proj_point_to_list_lemma: p:S.proj_point ->
-  Lemma (point_inv_list (proj_point_to_list p) /\ point_eval_list (proj_point_to_list p) == p)
 
 let proj_point_to_list_lemma p =
   proj_point_to_list_fits p;
